Remove more clutter and rename a bit

examples/tutorial/5-wp/tutorialExtra2_wpScript.sml
@@ -49,15 +49,15 @@ val get_2  = bconst ``2w:word64``;
 (* =============================================================== *)
 
 (* overall contract is_even *)
-val bir_ieo_ev_pre_def = Define `bir_ieo_ev_pre v1 =
+val bir_ieo_pre_def = Define `bir_ieo_pre v1 =
 ^(beq (get_n, get_v1))
 `;
 
-val bir_ieo_ev_post_yes_def = Define `bir_ieo_ev_post_yes v1 =
+val bir_ieo_post_even_def = Define `bir_ieo_post_even v1 =
 ^(beq (bmod (get_v1, get_2), get_0))
 `;
 
-val bir_ieo_ev_post_no_def = Define `bir_ieo_ev_post_no v1 =
+val bir_ieo_post_odd_def = Define `bir_ieo_post_odd v1 =
 ^(beq (bmod (get_v1, get_2), get_1))
 `;
 
@@ -90,8 +90,8 @@ val bir_ieo_sec_iseven_exit_pre_def = Define `bir_ieo_sec_iseven_exit_pre v1 =
 `;
 
 
-(* section is_even post *)
-val bir_ieo_sec_iseven_post_def = Define `bir_ieo_sec_iseven_post v1 v =
+(* section is_even loop post *)
+val bir_ieo_sec_iseven_loop_post_def = Define `bir_ieo_sec_iseven_loop_post v1 v =
 \l. if l = BL_Address (Imm32 0x000w) then
        (BExp_BinExp BIExp_And (bir_ieo_invariant v1)
                   (BExp_BinExp BIExp_And
@@ -105,9 +105,9 @@ val bir_ieo_sec_iseven_post_def = Define `bir_ieo_sec_iseven_post v1 v =
 (* section is_even exit post *)
 val bir_ieo_sec_iseven_exit_post_def = Define `bir_ieo_sec_iseven_exit_post v1 =
 \l. if l = BL_Address (Imm32 0x200w) then
-      bir_ieo_ev_post_yes v1
+      bir_ieo_post_even v1
     else if l = BL_Address (Imm32 0x204w) then
-      bir_ieo_ev_post_no v1
+      bir_ieo_post_odd v1
     else
       bir_exp_false
 `;
@@ -123,10 +123,10 @@ val bir_ieo_sec_iseven_exit_post_def = Define `bir_ieo_sec_iseven_exit_post v1 =
 val prefix = "bir_ieo_sec_iseven_loop_";
 val first_block_label_tm = ``BL_Address (Imm32 0x000w)``;
 val ending_set =  ``{BL_Address (Imm32 0x000w); BL_Address (Imm32 0x200w); BL_Address (Imm32 0x204w)}``;
-val postcond_tm = ``bir_ieo_sec_iseven_post v1 v``;
+val postcond_tm = ``bir_ieo_sec_iseven_loop_post v1 v``;
 
-val defs = [bprog_is_even_odd_def, bir_ieo_sec_iseven_post_def,
-            bir_ieo_ev_post_no_def, bir_ieo_ev_post_yes_def,
+val defs = [bprog_is_even_odd_def, bir_ieo_sec_iseven_loop_post_def,
+            bir_ieo_post_odd_def, bir_ieo_post_even_def,
             bir_ieo_invariant_def, bir_ieo_condition_def, bir_ieo_variant_def,
             bir_exp_false_def, BType_Bool_def];
 
@@ -148,7 +148,7 @@ val ending_set =  ``{BL_Address (Imm32 0x000w); BL_Address (Imm32 0x200w); BL_Ad
 val postcond_tm = ``bir_ieo_sec_iseven_exit_post v1``;
 
 val defs = [bprog_is_even_odd_def, bir_ieo_sec_iseven_exit_post_def,
-            bir_ieo_ev_post_no_def, bir_ieo_ev_post_yes_def, bir_ieo_invariant_def,
+            bir_ieo_post_odd_def, bir_ieo_post_even_def, bir_ieo_invariant_def,
             bir_exp_false_def, BType_Bool_def];
 
 val (bir_ieo_sec_iseven_exit_ht, bir_ieo_sec_iseven_exit_wp_tm) =
